wip

ulib/LowStar.BufferView.fsti
@@ -41,28 +41,6 @@ let length (#a #b: _) (vb:buffer_view a b)
   = length (as_buffer vb) / View?.n (get_view vb)
 
 module HS=FStar.HyperStack
-
-let rec get_seq
-        #a #b
-        (v:view a b)
-        (as:Seq.seq a{Seq.length as % View?.n v == 0})
-      : GTot (bs:Seq.seq b{Seq.length bs = Seq.length as / View?.n v})
-             (decreases (Seq.length as))
-      = let n = View?.n v in
-        if Seq.length as = 0
-        then Seq.createEmpty #b
-        else let prefix, suffix = Seq.split as n in
-             assert (Seq.length suffix = Seq.length as - n);
-             FStar.Math.Lemmas.lemma_mod_sub (Seq.length as) n 1;
-             let tail = get_seq v suffix in
-             Seq.cons (View?.get v prefix) tail
-
-let as_seq (#a #b: _) (h:HS.mem) (vb:buffer_view a b)
-  : GTot (Seq.lseq b (length vb))
-  = let s0 = as_seq h (as_buffer vb) in
-    let v = get_view vb in
-    get_seq v s0
-
 module B=LowStar.Buffer
 
 #reset-options "--max_fuel 0 --max_ifuel 1"
@@ -72,6 +50,12 @@ let view_indexing (#a #b: _) (vb:buffer_view a b) (i:nat{i < length vb})
            n <= length vb * n - i * n)
   = let n = View?.n (get_view vb) in
     FStar.Math.Lemmas.distributivity_add_left (length vb) (-i) n
+
+let lt_leq_mul (min:nat) (max:nat{min < max}) (n:nat) :
+  Lemma (FStar.Mul.(min * n + n <= max * n)) =
+  let open FStar.Mul in
+  assert ((min * n) + n = (min + 1) * n);
+  assert ((min * n) + n <= max * n)
 
 let split_at_i (#a #b: _) (vb:buffer_view a b) (i:nat{i < length vb}) (h:HS.mem)
     : GTot (frags:
@@ -128,7 +112,8 @@ let sel_upd1 (#a #b:_) (vb:buffer_view a b) (i:nat{i < length vb}) (x:b) (h:HS.m
                          as'' suffix';
     assert (as' == as'')
 
-#set-options "--z3rlimit_factor 3"
+
+#reset-options "--max_fuel 0 --max_ifuel 1"
 let sel_upd2 (#a #b:_) (vb:buffer_view a b) (i:nat{i < length vb}) (j:nat{j < length vb /\ i<>j}) (x:b) (h:HS.mem{live h vb})
   : Lemma (sel vb j (upd vb i x h) == sel vb j h)
   = let open FStar.Mul in
@@ -141,68 +126,74 @@ let sel_upd2 (#a #b:_) (vb:buffer_view a b) (i:nat{i < length vb}) (j:nat{j < le
     let min = if i < j then i else j in
     let max = if i < j then j else i in
     let n = View?.n v in
-    assert (min < max);
-    assume ((min * n) + n <= max * n);
-    let p0, min0, m0, max0, t0 =
-        Seq.slice s0 0 (min * n),
+    lt_leq_mul min max n;
+    let min0, max0 =
         Seq.slice s0 (min * n) ((min * n) + n),
-        Seq.slice s0 ((min * n) + n) (max * n),
-        Seq.slice s0 (max * n) ((max * n) + n),
-        Seq.slice s0 ((max * n) + n) (length vb * n)
+        Seq.slice s0 (max * n) ((max * n) + n)
     in
-    let p1, min1, m1, max1, t1 =
-        Seq.slice s1 0 (min * n),
+    let _, s_j, _ = split_at_i vb j h in
+    let min1, max1 =
         Seq.slice s1 (min * n) ((min * n) + n),
-        Seq.slice s1 ((min * n) + n) (max * n),
-        Seq.slice s1 (max * n) ((max * n) + n),
-        Seq.slice s1 ((max * n) + n) (length vb * n)
+        Seq.slice s1 (max * n) ((max * n) + n)
     in
-    admit()
+    let _, s_j', _ = split_at_i vb j h' in
+    let prefix, s_i, suffix = split_at_i vb i h in
+    B.g_upd_seq_as_seq (as_buffer vb) (prefix `Seq.append` (View?.put v x `Seq.append` suffix)) h;
+    if i < j
+    then begin
+      assert (Seq.equal max0 s_j);
+      assert (Seq.equal max1 s_j');
+      assert (Seq.equal s_j s_j')
+    end
+    else begin
+      assert (Seq.equal min0 s_j);
+      assert (Seq.equal min1 s_j');
+      assert (Seq.equal s_j s_j')
+    end
 
+let rec as_seq' (#a #b: _) (h:HS.mem) (vb:buffer_view a b) (i:nat{i <= length vb})
+  : GTot (Seq.lseq b (length vb - i))
+         (decreases (length vb - i))
+  = let v = get_view vb in
+    if i = length vb
+    then Seq.createEmpty
+    else let _ = view_indexing vb i in
+         let _, s_i, suffix = split_at_i vb i h in
+         View?.get v s_i `Seq.cons` as_seq' h vb (i + 1)
 
+let as_seq (#a #b: _) (h:HS.mem) (vb:buffer_view a b) =
+    as_seq' h vb 0
 
-    let prefix, as, suffix = split_at_i vb i h in
-    let as' = View?.put v x in
-    let s' = B.as_seq h' (as_buffer vb) in
-    B.g_upd_seq_as_seq (as_buffer vb) (prefix `Seq.append` (as' `Seq.append` suffix)) h;
-    assert (s' == prefix `Seq.append` (as' `Seq.append` suffix));
-    let prefix', as'', suffix' = split_at_i vb i h' in
-    assert (s' == prefix' `Seq.append` (as'' `Seq.append` suffix'));
-    Seq.lemma_append_inj prefix  (as' `Seq.append` suffix)
-                         prefix' (as'' `Seq.append` suffix');
-    Seq.lemma_append_inj as' suffix
-                         as'' suffix';
-    assert (prefix == prefix');
-    assert (suffix == suffix');
-    let prefix'', res, suffix'' = split_at_i vb j h' in
+#set-options "--max_fuel 1 --max_ifuel 1"
+let as_seq_sel (#a #b: _) (h:HS.mem) (vb:buffer_view a b) (i:nat{i < length vb})
+    : Lemma (ensures (sel vb i h == Seq.index (as_seq h vb) i))
+    =
+      let rec as_seq'_as_seq' (#a #b: _)
+                              (h:HS.mem)
+                              (vb:buffer_view a b)
+                              (j:nat)
+                              (i:nat{j + i < length vb})
+        : Lemma (ensures (Seq.index (as_seq' h vb j) i == Seq.index (as_seq' h vb (j + i)) 0))
+                (decreases i)
+        = if i = 0 then () else as_seq'_as_seq' h vb (j + 1) (i - 1)
+      in
+      as_seq'_as_seq' h vb 0 i
 
-    ()
+#set-options "--max_fuel 0 --max_ifuel 1"
+let get_sel (#a #b: _) (h:HS.mem) (vb:buffer_view a b) (i:nat{i < length vb})
+    : Lemma (ensures (let open FStar.Mul in
+                      let v = get_view vb in
+                      let n = View?.n v in
+                      view_indexing vb i;
+                      sel vb i h ==
+                      View?.get v (Seq.slice (B.as_seq h (as_buffer vb)) (i * n) (i * n + n))))
+    = ()
 
-
-val sel_view (#a #b: _) (vb:buffer_view a b) (i:nat{i < length vb}) (h:HS.mem)
-   : Lemma (let open FStar.Mul in
-            let as = B.as_seq h (as_buffer vb) in
-            let v = get_view vb in
-            let start = View?.n v * i in
-            let finish = start + View?.n v in
-            let a  = Seq.slice as start finish in
-            sel vb i h == View?.get v a)
-   = admit()Seq.index (as_seq h vb) i
-
-let sel_vew #a #b (vb:buffer_view a b)
-
-
-#set-options "--z3rlimit_factor 2"
-let upd (#a #b: _) (vb:buffer_view a b) (i:nat{i < length vb}) (x:b) (h:HS.mem{live h vb})
-  : GTot HS.mem
-  = let open FStar.Mul in
-    let s0 = B.as_seq h (as_buffer vb) in
-    let v = get_view vb in
-    let n = View?.n v in
-    let j = i * n in
-    let prefix, suffix = Seq.split s0 j in
-    assert (Seq.length suffix = length vb * n - (i * n));
-    FStar.Math.Lemmas.distributivity_add_left (length vb) (-i) n;
-    let _, tail = Seq.split suffix n in
-    let s1 = Seq.append prefix (Seq.append (View?.put v x) tail) in
-    B.g_upd_seq (as_buffer vb) s1 h
+let put_sel (#a #b: _) (h:HS.mem) (vb:buffer_view a b) (i:nat{i < length vb})
+    : Lemma (ensures (let open FStar.Mul in
+                      let v = get_view vb in
+                      let n = View?.n v in
+                      view_indexing vb i;
+                      View?.put v (sel vb i h) ==
+                      Seq.slice (B.as_seq h (as_buffer vb)) (i * n) (i * n + n)))
+    = get_sel h vb i
